# Logic

- **[L1]** (P ⇔ Q) ⇔ (P ⇒ Q) ∧ (Q ⇒ P)
- **[L2]** P ∧ Q ⇔ Q ∧ P
- **[L3]** P ∧ (Q ∧ R) ⇔ (P ∧ Q) ∧ R
- **[L4]** P ∨ Q ⇔ Q ∨ P
- **[L5]** P ∨ (Q ∨ R) ⇔ (P ∨ Q) ∨ R
- **[L6]** P ∧ t ⇔ P
- **[L7]** P ∨ f ⇔ P
- **[L8]** P ∧ f ⇔ f
- **[L9]** P ∨ t ⇔ t
- **[L10]** P ∧ ¬P ⇔ f
- **[L11]** P ∨ ¬P ⇔ t
- **[L12]** P ⇒ f ⇔ ¬P
- **[L13]** P ⇒ Q ⇔ ¬P ∨ Q
- **[L14]** ¬¬P ⇔ P
- **[L15]** P ∨ (Q ∧ R) ⇔ (P ∨ Q) ∧ (P ∨ R)
- **[L16]** P ∧ (Q ∨ R) ⇔ (P ∧ Q) ∨ (P ∧ R)
- **[L17]** ¬(P ∧ Q) ⇔ ¬P ∨ ¬Q
- **[L18]** ¬(P ∨ Q) ⇔ ¬P ∧ ¬Q
- **[L19]** ∃x ¬P(x) ⇔ ¬(∀x P(x))
- **[L20]** ∀x ¬P(x) ⇔ ¬(∃x P(x))
- **[L21]** (P ∧ Q) ⇒ R ⇔ P ⇒ (Q ⇒ R)
- **[L22]** ¬t ⇔ f

# Arithmetic

### ∀ x ∈ ℤ, y ∈ ℤ, z ∈ ℤ

- **[A1]** (x < y) ∨ (x = y) ∨ (x > y) ⇔ t
- **[A2]** (x < y) ⇔ ¬(x = y) ∧ ¬(x > y)
- **[A3]** (x = y) ⇔ ¬(x < y) ∧ ¬(x > y)
- **[A4]** (x > y) ⇔ ¬(x < y) ∧ ¬(x = y)
- **[A5]** (x <= y) ⇔ (x < y) ∨ (x = y)
- **[A6]** (x >= y) ⇔ (x > y) ∨ (x = y)
- **[A7]** (x < y) ∧ (y < z) ⇒ (x < z)
- **[A8]** (x = y) ∧ (y = z) ⇒ (x = z)
- **[A9]** (x > y) ∧ (y > z) ⇒ (x > z)
- **[A10]** (x < y) ∧ (y < z) ∧ (z < x) ⇔ f
